Revamped BitMachine evaluation to produce a thrist of states the execution passes through. This should be helpful when describing the static analysis.

Coq/Simplicity/BitMachine.v
@@ -1,57 +1,10 @@
 Require Import PeanoNat.
 Require Import Util.List.
 Require Import Util.Option.
+Require Import Util.Thrist.
+Require Import Eqdep_dec.
 
 Definition Cell := option bool.
-
-Module MachineCode.
-
-Inductive T : Set :=
-| End : T
-| Crash : T
-| Write : bool -> T -> T
-| Copy : nat -> T -> T
-| Skip : nat -> T -> T
-| Fwd : nat -> T -> T
-| Bwd : nat -> T -> T
-| NewFrame : nat -> T -> T
-| MoveFrame : T -> T
-| DropFrame : T -> T
-| Read : T -> T -> T.
-
-Fixpoint append (x y : T) : T :=
-match x with
-| End => y
-| Crash => Crash
-| Write b k => Write b (append k y)
-| Copy n k => Copy n (append k y)
-| Skip n k => Skip n (append k y)
-| Fwd n k => Fwd n (append k y)
-| Bwd n k => Bwd n (append k y)
-| NewFrame n k => NewFrame n (append k y)
-| MoveFrame k => MoveFrame (append k y)
-| DropFrame k => DropFrame (append k y)
-| Read k0 k1 => Read (append k0 y) (append k1 y)
-end.
-
-End MachineCode.
-Bind Scope mc_scope with MachineCode.T.
-
-Definition crash : MachineCode.T := MachineCode.Crash.
-Definition write (b : bool) : MachineCode.T := MachineCode.Write b MachineCode.End.
-Definition copy (n : nat) : MachineCode.T := MachineCode.Copy n MachineCode.End.
-Definition skip (n : nat) : MachineCode.T := MachineCode.Skip n MachineCode.End.
-Definition fwd (n : nat) : MachineCode.T := MachineCode.Fwd n MachineCode.End.
-Definition bwd (n : nat) : MachineCode.T := MachineCode.Bwd n MachineCode.End.
-Definition newFrame (n : nat) : MachineCode.T := MachineCode.NewFrame n MachineCode.End.
-Definition moveFrame : MachineCode.T := MachineCode.MoveFrame MachineCode.End.
-Definition dropFrame : MachineCode.T := MachineCode.DropFrame MachineCode.End.
-Definition read (k0 k1 : MachineCode.T) : MachineCode.T := MachineCode.Read k0 k1.
-
-Notation "p ;; q" := (MachineCode.append p q) (at level 40, left associativity) : mc_scope.
-
-Definition nop : MachineCode.T := MachineCode.End.
-Definition bump n p : MachineCode.T := fwd n ;; p ;; bwd n.
 
 (* Write-only frames are append only.  We represent the frame by, writeData,
  * the list of cells before the frame's cursor, and by writeEmpty, which
@@ -102,75 +55,6 @@ Definition setFrame l :=
   ; nextData := l
   |}.
 
-Definition resetFrame wf :=
-match writeEmpty wf with
-| O => Some (setFrame (rev (writeData wf)))
-| S _ => None
-end.
-
-Definition advFrame f :=
-match nextData f with
-| nil => None
-| hd :: tl => Some {| prevData := hd :: prevData f; nextData := tl |}
-end.
-
-Definition retFrame f :=
-match prevData f with
-| nil => None
-| hd :: tl => Some {| prevData := tl; nextData := hd :: nextData f |}
-end.
-
-Fixpoint fwdFrame n f :=
-match n with
-| O => Some f
-| (S m) => option_bind (fwdFrame m) (advFrame f)
-end.
-
-Fixpoint bwdFrame n f :=
-match n with
-| O => Some f
-| (S m) => option_bind (bwdFrame m) (retFrame f)
-end.
-
-Definition sliceFrame n f :=
-if Nat.leb n (length (nextData f))
-then Some (firstn n (nextData f))
-else None.
-
-Lemma fwdFrame_correct l : forall pd nd,
-   fwdFrame (length l) {| prevData := pd; nextData := l ++ nd |}
- = Some {| prevData := rev l ++ pd; nextData := nd |}.
-Proof.
-induction l;[reflexivity|].
-intros pd nd.
-cbn.
-rewrite IHl, <- app_assoc.
-reflexivity.
-Qed.
-
-Lemma bwdFrame_correct l : forall pd nd,
-   bwdFrame (length l) {| prevData := l ++ pd; nextData := nd |}
- = Some {| prevData := pd; nextData := rev l ++ nd |}.
-Proof.
-induction l;[reflexivity|].
-intros pd nd.
-cbn.
-rewrite IHl, <- app_assoc.
-reflexivity.
-Qed.
-
-Lemma sliceFrame_correct l pd nd :
-  sliceFrame (length l) {| prevData := pd; nextData := l ++ nd |} = Some l.
-Proof.
-unfold sliceFrame; cbn.
-rewrite app_length.
-case (Nat.leb_spec0 _ _);[intros _|intros []; auto with *].
-rewrite (plus_n_O (length l)), firstn_app_2, firstn_O, app_nil_r.
-reflexivity.
-Qed.
-
-Definition readFromFrame f := hd None (nextData f).
-
 (* The full state of the Bit Machine is captured by a list of inactive
  * read-only and write-only frames.  The top of the two stacks are held in the
  * activeReadFrame and activeWriteFrame.  This ensures that both stacks are
@@ -183,27 +67,16 @@ Record State :=
  ; inactiveWriteFrames : list WriteFrame
  }.
 
+Lemma State_dec (x y : State) : {x = y} + {x <> y}.
+Proof.
+repeat (decide equality).
+Qed.
+
 Definition stateSize s :=
   fold_right plus 0 (map readSize (inactiveReadFrames s)) +
   readSize (activeReadFrame s) +
   writeSize (activeWriteFrame s) +
   fold_right plus 0 (map writeSize (inactiveWriteFrames s)).
-
-Definition oModActiveReadFrame f s : option State :=
-  option_map (fun x =>
-    {| inactiveReadFrames := inactiveReadFrames s
-     ; activeReadFrame := x
-     ; activeWriteFrame := activeWriteFrame s
-     ; inactiveWriteFrames := inactiveWriteFrames s
-     |}) (f (activeReadFrame s)).
-
-Definition oModActiveWriteFrame f s : option State :=
-  option_map (fun x =>
-    {| inactiveReadFrames := inactiveReadFrames s
-     ; activeReadFrame := activeReadFrame s
-     ; activeWriteFrame := x
-     ; inactiveWriteFrames := inactiveWriteFrames s
-     |}) (f (activeWriteFrame s)).
 
 (* Logically, the state of the Bit Machine is commonly divided between the part
  * of the state that we are focused on and the rest of state.  The focused part
@@ -274,151 +147,582 @@ rewrite Plus.plus_assoc.
 reflexivity.
 Qed.
 
-Module State.
-
-Definition write b :=
-  oModActiveWriteFrame (writeToFrame (Some b)).
-
-Definition copy n s :=
-  oModActiveWriteFrame (fun wf => option_bind (fun l => writeListFrame l wf) (sliceFrame n (activeReadFrame s))) s.
-
-Definition skip n :=
-  oModActiveWriteFrame (writeListFrame (repeat None n)).
-
-Definition fwd n :=
-  oModActiveReadFrame (fwdFrame n).
-
-Definition bwd n :=
-  oModActiveReadFrame (bwdFrame n).
-
-Definition newFrame n s :=
-  Some {| inactiveReadFrames := inactiveReadFrames s
-        ; activeReadFrame := activeReadFrame s
-        ; activeWriteFrame := newWriteFrame n
-        ; inactiveWriteFrames := activeWriteFrame s :: inactiveWriteFrames s
-        |}.
-
-Definition moveFrame s :=
-match inactiveWriteFrames s with
-| nil => None
-| hd :: tl => option_map (fun x =>
-  {| inactiveReadFrames := activeReadFrame s :: inactiveReadFrames s
-   ; activeReadFrame := x
-   ; activeWriteFrame := hd
-   ; inactiveWriteFrames := tl
-   |}) (resetFrame (activeWriteFrame s))
-end.
-
-Definition dropFrame s :=
-match inactiveReadFrames s with
-| nil => None
-| hd :: tl => Some
-  {| inactiveReadFrames := tl
-   ; activeReadFrame := hd
-   ; activeWriteFrame := activeWriteFrame s
-   ; inactiveWriteFrames := inactiveWriteFrames s
-   |}
-end.
-
-Lemma skip_correct n m l0 l1 (ctx : Context) :
-  skip n (fillContext ctx {| readLocalState := l0
-                           ; writeLocalState :=
-                             {| writeData := l1
-                              ; writeEmpty := n + m
-                           |} |})
-= Some (fillContext ctx {| readLocalState := l0
-                         ; writeLocalState :=
-                           {| writeData := repeat None n ++ l1
-                            ; writeEmpty := m
-                         |} |}).
-Proof.
-unfold skip, fillContext, oModActiveWriteFrame.
-cbn.
-revert l1.
-induction n;[reflexivity|].
-intros l1.
-cbn.
-set (wd := writeData (activeWriteFrame ctx)).
-change (None :: (repeat None n ++ l1) ++ wd) with ((repeat None (S n) ++ l1) ++ wd).
-rewrite <- repeat_S_tail.
-rewrite <- (app_assoc _ _ l1).
-apply (IHn (None :: l1)).
-Qed.
-
-Lemma copy_correct (l : list Cell) (ctx : Context) :
-  copy (length l) (fillContext ctx {| readLocalState := l
-                                    ; writeLocalState := newWriteFrame (length l)
-                                    |})
-= Some (fillContext ctx {| readLocalState := l
-                         ; writeLocalState := fullWriteFrame l
-                         |}).
-Proof.
-unfold copy, fillContext, oModActiveWriteFrame; cbn.
-rewrite sliceFrame_correct; cbn.
-set (rf := (Build_ReadFrame _ _)); clearbody rf.
-set (wd := writeData _); clearbody wd; revert wd.
-induction l;[reflexivity|];intros wd; cbn.
-rewrite IHl, <- app_assoc.
-reflexivity.
-Qed.
-
-End State.
-
-Fixpoint runMachine (p : MachineCode.T) s : option State :=
-match p with
-| MachineCode.End => Some s
-| MachineCode.Crash => None
-| MachineCode.Write b k => option_bind (runMachine k) (State.write b s)
-| MachineCode.Copy n k => option_bind (runMachine k) (State.copy n s)
-| MachineCode.Skip n k => option_bind (runMachine k) (State.skip n s)
-| MachineCode.Fwd n k => option_bind (runMachine k) (State.fwd n s)
-| MachineCode.Bwd n k => option_bind (runMachine k) (State.bwd n s)
-| MachineCode.NewFrame n k => option_bind (runMachine k) (State.newFrame n s)
-| MachineCode.MoveFrame k => option_bind (runMachine k) (State.moveFrame s)
-| MachineCode.DropFrame k => option_bind (runMachine k) (State.dropFrame s)
-| MachineCode.Read k0 k1 => option_bind
-  (fun b : bool => if b then runMachine k1 s else runMachine k0 s)
-  (readFromFrame (activeReadFrame s))
-end.
-
-Lemma runMachine_append p q s :
-  runMachine (p ;; q) s = option_bind (runMachine q) (runMachine p s).
-Proof.
-revert q s; induction p; intros q s; try reflexivity;
- simpl; rewrite option_bind_assoc; apply option_bind_ext; auto.
-intros [|]; auto.
-Qed.
-
-Definition bumpContext (ctx : Context) l : Context :=
+Definition fillReadFrame (ctx : Context) (h : ReadFrame) : State :=
  {| inactiveReadFrames := inactiveReadFrames ctx
   ; activeReadFrame :=
-    {| prevData := rev l ++ prevData (activeReadFrame ctx)
-     ; nextData := nextData (activeReadFrame ctx)
-     |}
+      {| prevData := prevData h ++ prevData (activeReadFrame ctx)
+       ; nextData := nextData h ++ nextData (activeReadFrame ctx)
+       |}
   ; activeWriteFrame := activeWriteFrame ctx
   ; inactiveWriteFrames := inactiveWriteFrames ctx
   |}.
 
-Definition bumpLocalState l : LocalState := {| readLocalState := l; writeLocalState := newWriteFrame 0 |}.
+Module MachineCode.
 
-Lemma runMachine_bump ctx l ls1 ls2 p :
-    runMachine p (fillContext (bumpContext ctx l) ls1) = Some (fillContext (bumpContext ctx l) ls2)
- -> runMachine (bump (length l) p) (fillContext ctx (appendLocalState ls1 (bumpLocalState l)))
-    = Some (fillContext ctx (appendLocalState ls2 (bumpLocalState l))).
+Inductive T : State -> State -> Set :=
+| NewFrame : forall n ctx,
+    T ctx
+      {| inactiveReadFrames := inactiveReadFrames ctx
+       ; activeReadFrame := activeReadFrame ctx
+       ; activeWriteFrame := newWriteFrame n
+       ; inactiveWriteFrames := activeWriteFrame ctx :: inactiveWriteFrames ctx
+       |}
+| MoveFrame : forall l ctx,
+    T {| inactiveReadFrames := inactiveReadFrames ctx
+       ; activeReadFrame := activeReadFrame ctx
+       ; activeWriteFrame := fullWriteFrame l
+       ; inactiveWriteFrames := activeWriteFrame ctx :: inactiveWriteFrames ctx
+       |}
+      {| inactiveReadFrames := activeReadFrame ctx :: inactiveReadFrames ctx
+       ; activeReadFrame := setFrame l
+       ; activeWriteFrame := activeWriteFrame ctx
+       ; inactiveWriteFrames := inactiveWriteFrames ctx
+       |}
+| DropFrame : forall rf ctx,
+    T {| inactiveReadFrames := activeReadFrame ctx :: inactiveReadFrames ctx
+       ; activeReadFrame := rf
+       ; activeWriteFrame := activeWriteFrame ctx
+       ; inactiveWriteFrames := inactiveWriteFrames ctx
+       |}
+      ctx
+| Write : forall b ctx,
+    T (fillContext ctx {| readLocalState := nil
+                        ; writeLocalState := newWriteFrame 1
+                        |})
+      (fillContext ctx {| readLocalState := nil
+                        ; writeLocalState := fullWriteFrame (Some b :: nil)
+                        |})
+| Skip : forall n ctx,
+    T (fillContext ctx {| readLocalState := nil
+                        ; writeLocalState := newWriteFrame n
+                        |})
+      (fillContext ctx {| readLocalState := nil
+                        ; writeLocalState := fullWriteFrame (repeat None n)
+                        |})
+| Copy : forall l ctx,
+    T (fillContext ctx {| readLocalState := l
+                        ; writeLocalState := newWriteFrame (length l)
+                        |})
+      (fillContext ctx {| readLocalState := l
+                        ; writeLocalState := fullWriteFrame l
+                        |})
+| Fwd : forall l ctx,
+    T (fillReadFrame ctx {| prevData := nil
+                          ; nextData := l
+                          |})
+      (fillReadFrame ctx {| prevData := rev l
+                          ; nextData := nil
+                          |})
+| Bwd : forall l ctx,
+    T (fillReadFrame ctx {| prevData := rev l
+                          ; nextData := nil
+                          |})
+      (fillReadFrame ctx {| prevData := nil
+                          ; nextData := l
+                          |}).
+
+End MachineCode.
+
+Definition MoveFrame_ctx s :
+  option { lctx : list Cell * Context | let (l, ctx) := lctx in s =
+      {| inactiveReadFrames := inactiveReadFrames ctx
+       ; activeReadFrame := activeReadFrame ctx
+       ; activeWriteFrame := fullWriteFrame l
+       ; inactiveWriteFrames := activeWriteFrame ctx :: inactiveWriteFrames ctx
+       |}}.
+destruct s as [irf arf [l n] [|awf iwf]].
+ exact None.
+destruct n as [|n];[|exact None].
+pose (ctx := {| inactiveReadFrames := irf
+              ; activeReadFrame := arf
+              ; activeWriteFrame := awf
+              ; inactiveWriteFrames := iwf
+              |}).
+left.
+exists (rev l, ctx).
+unfold fullWriteFrame.
+abstract (rewrite rev_involutive; reflexivity).
+Defined.
+
+Lemma MoveFrame_ctx_correct l ctx : MoveFrame_ctx
+ {| inactiveReadFrames := inactiveReadFrames ctx
+  ; activeReadFrame := activeReadFrame ctx
+  ; activeWriteFrame := fullWriteFrame l
+  ; inactiveWriteFrames := activeWriteFrame ctx :: inactiveWriteFrames ctx
+  |} = Some (exist _ (l, ctx) (refl_equal _)).
+Proof.
+cbn.
+set (H := (MoveFrame_ctx_subproof _ _ _ _ _)).
+generalize H; clear H.
+rewrite (rev_involutive l).
+apply (K_dec_set State_dec).
+destruct ctx as [irf arf awf iwf].
+reflexivity.
+Qed.
+
+Definition DropFrame_ctx s :
+  option { rfctx : ReadFrame * Context | let (rf, ctx) := rfctx in s =
+      {| inactiveReadFrames := activeReadFrame ctx :: inactiveReadFrames ctx
+       ; activeReadFrame := rf
+       ; activeWriteFrame := activeWriteFrame ctx
+       ; inactiveWriteFrames := inactiveWriteFrames ctx
+       |}}.
+destruct s as [[|arf irf] rf awf iwf].
+ exact None.
+pose (ctx := {| inactiveReadFrames := irf
+              ; activeReadFrame := arf
+              ; activeWriteFrame := awf
+              ; inactiveWriteFrames := iwf
+              |}).
+left.
+exists (rf, ctx).
+reflexivity.
+Defined.
+
+Lemma DropFrame_ctx_correct rf ctx : DropFrame_ctx
+ {| inactiveReadFrames := activeReadFrame ctx :: inactiveReadFrames ctx
+  ; activeReadFrame := rf
+  ; activeWriteFrame := activeWriteFrame ctx
+  ; inactiveWriteFrames := inactiveWriteFrames ctx
+  |} = Some (exist _ (rf, ctx) (refl_equal _)).
+Proof.
+destruct ctx; reflexivity.
+Qed.
+
+Definition Write_ctx s :
+  option { ctx : Context | s =
+    fillContext ctx {| readLocalState := nil
+                     ; writeLocalState := newWriteFrame 1
+                     |}}.
+destruct s as [irf [rp rn] [wd [|we]] iwf].
+ exact None.
+left.
+pose (ctx := {| inactiveReadFrames := irf
+              ; activeReadFrame := {| prevData := rp; nextData := rn |}
+              ; activeWriteFrame := {| writeData := wd; writeEmpty := we |}
+              ; inactiveWriteFrames := iwf
+              |}).
+exists ctx.
+reflexivity.
+Defined.
+
+Lemma Write_ctx_correct ctx : Write_ctx
+  (fillContext ctx {| readLocalState := nil
+                    ; writeLocalState := newWriteFrame 1
+                    |})
+  = Some (exist _ ctx (refl_equal _)).
+Proof.
+destruct ctx as [irf [rp rn] [wd we] iwf].
+reflexivity.
+Qed.
+
+Definition Skip_ctx n s :
+  option { ctx : Context | s =
+    fillContext ctx {| readLocalState := nil
+                     ; writeLocalState := newWriteFrame n
+                     |}}.
+destruct s as [irf [rp rn] [wd we] iwf].
+generalize (Nat.leb_spec n we).
+destruct (n <=? we);intros H;[|exact None].
+left.
+pose (ctx := {| inactiveReadFrames := irf
+              ; activeReadFrame := {| prevData := rp; nextData := rn |}
+              ; activeWriteFrame := {| writeData := wd; writeEmpty := we - n |}
+              ; inactiveWriteFrames := iwf
+              |}).
+exists ctx.
+abstract (
+  unfold fillContext; cbn;
+  inversion_clear H as [Hn|];
+  rewrite <- (Minus.le_plus_minus _ _ Hn);
+  reflexivity).
+Defined.
+
+Lemma Skip_ctx_correct n ctx : Skip_ctx n
+  (fillContext ctx {| readLocalState := nil
+                    ; writeLocalState := newWriteFrame n
+                    |})
+  = Some (exist _ ctx (refl_equal _)).
+Proof.
+cbn.
+destruct (Nat.leb_spec n (n + writeEmpty (activeWriteFrame ctx))) as [H0|H0];
+ [|elim (Lt.lt_not_le _ _ H0); auto with arith].
+set (H := (Skip_ctx_subproof _ _ _ _ _ _ _ _)).
+generalize H; clear H.
+rewrite Minus.minus_plus.
+apply (K_dec_set State_dec).
+destruct ctx as [irf [rp rn] [wd we] iwf].
+reflexivity.
+Qed.
+
+Definition Copy_ctx n s :
+  option { lctx : list Cell * Context | let (l, ctx) := lctx in n = length l /\ s =
+    fillContext ctx {| readLocalState := l
+                     ; writeLocalState := newWriteFrame (length l)
+                     |}}.
+destruct s as [irf [rp rn] [wd we] iwf].
+generalize (Nat.leb_spec n we).
+destruct (n <=? we);intros Hwe;[|exact None].
+generalize (Nat.leb_spec n (length rn)).
+destruct (n <=? length rn);intros Hrn;[|exact None].
+left.
+pose (ctx := {| inactiveReadFrames := irf
+              ; activeReadFrame := {| prevData := rp; nextData := skipn n rn |}
+              ; activeWriteFrame := {| writeData := wd; writeEmpty := we - n |}
+              ; inactiveWriteFrames := iwf
+              |}).
+exists (firstn n rn, ctx).
+split.
+- abstract
+(inversion_clear Hrn as [H|];
+ rewrite (firstn_length_le _ H);
+ reflexivity).
+- abstract
+(inversion_clear Hrn as [H|];
+ rewrite (firstn_length_le _ H);
+ clear H;
+ unfold fillContext; cbn;
+ inversion_clear Hwe as [H|];
+ rewrite firstn_skipn, <- (Minus.le_plus_minus _ _ H);
+ reflexivity).
+Defined.
+
+Lemma Copy_ctx_correct l ctx : Copy_ctx (length l)
+  (fillContext ctx {| readLocalState := l
+                    ; writeLocalState := newWriteFrame (length l)
+                    |})
+  = Some (exist _ (l, ctx) (conj (refl_equal _) (refl_equal _))).
+Proof.
+cbn.
+destruct (Nat.leb_spec (length l) (length l + writeEmpty (activeWriteFrame ctx))) as [H0|H0];
+ [|elim (Lt.lt_not_le _ _ H0); auto with arith].
+destruct (Nat.leb_spec (length l) (length (l ++ nextData (activeReadFrame ctx)))) as [H1|H1];
+ [|elim (Lt.lt_not_le _ _ H1); rewrite app_length; auto with arith].
+set (H := (Copy_ctx_subproof _ _ _)).
+generalize H; clear H.
+set (H := (Copy_ctx_subproof0 _ _ _ _ _ _ _ _ _)).
+generalize H; clear H.
+rewrite firstn_app, firstn_all, Nat.sub_diag; cbn.
+rewrite app_nil_r, Minus.minus_plus.
+replace (skipn (length l) _) with (nextData (activeReadFrame ctx))
+ by (apply (app_inv_head (firstn (length l) (l ++ nextData (activeReadFrame ctx))));
+     rewrite firstn_skipn, firstn_app, firstn_all, Nat.sub_diag; cbn;
+     rewrite app_nil_r; reflexivity).
+intros H; elim H using (K_dec_set State_dec); clear H.
+apply (K_dec_set Nat.eq_dec).
+destruct ctx as [irf [rp rn] [wd we] iwf].
+reflexivity.
+Qed.
+
+Definition Fwd_ctx n s :
+  option { lctx : list Cell * Context | let (l, ctx) := lctx in n = length l /\ s =
+    fillReadFrame ctx {| prevData := nil
+                       ; nextData := l
+                       |}}.
+destruct s as [irf [rp rn] awf iwf].
+generalize (Nat.leb_spec n (length rn)).
+destruct (n <=? length rn);intros Hrn;[|exact None].
+left.
+pose (ctx := {| inactiveReadFrames := irf
+              ; activeReadFrame := {| prevData := rp; nextData := skipn n rn |}
+              ; activeWriteFrame := awf
+              ; inactiveWriteFrames := iwf
+              |}).
+exists (firstn n rn, ctx).
+split.
+- abstract
+(inversion_clear Hrn as [H|];
+ rewrite (firstn_length_le _ H);
+ reflexivity).
+- abstract
+(unfold fillReadFrame; cbn;
+ inversion_clear Hrn as [H|];
+ rewrite firstn_skipn;
+ reflexivity).
+Defined.
+
+Lemma Fwd_ctx_correct l ctx : Fwd_ctx (length l)
+  (fillReadFrame ctx {| prevData := nil
+                      ; nextData := l
+                      |})
+  = Some (exist _ (l, ctx) (conj (refl_equal _) (refl_equal _))).
+Proof.
+cbn.
+destruct (Nat.leb_spec (length l) (length (l ++ nextData (activeReadFrame ctx)))) as [H0|H0];
+ [|elim (Lt.lt_not_le _ _ H0); rewrite app_length; auto with arith].
+set (H := (Fwd_ctx_subproof _ _ _)).
+generalize H; clear H.
+set (H := (Fwd_ctx_subproof0 _ _ _ _ _ _ _)).
+generalize H; clear H.
+rewrite firstn_app, firstn_all, Nat.sub_diag; cbn.
+rewrite app_nil_r.
+replace (skipn (length l) _) with (nextData (activeReadFrame ctx))
+ by (apply (app_inv_head (firstn (length l) (l ++ nextData (activeReadFrame ctx))));
+     rewrite firstn_skipn, firstn_app, firstn_all, Nat.sub_diag; cbn;
+     rewrite app_nil_r; reflexivity).
+intros H; elim H using (K_dec_set State_dec); clear H.
+apply (K_dec_set Nat.eq_dec).
+destruct ctx as [irf [rp rn] [wd we] iwf].
+reflexivity.
+Qed.
+
+Definition Bwd_ctx n s :
+  option { lctx : list Cell * Context | let (l, ctx) := lctx in n = length l /\ s =
+    fillReadFrame ctx {| prevData := rev l
+                       ; nextData := nil
+                       |}}.
+destruct s as [irf [rp rn] awf iwf].
+generalize (Nat.leb_spec n (length rp)).
+destruct (n <=? length rp);intros Hrp;[|exact None].
+left.
+pose (ctx := {| inactiveReadFrames := irf
+              ; activeReadFrame := {| prevData := skipn n rp; nextData := rn |}
+              ; activeWriteFrame := awf
+              ; inactiveWriteFrames := iwf
+              |}).
+exists (rev (firstn n rp), ctx).
+split.
+- abstract
+(inversion_clear Hrp as [H|];
+ rewrite rev_length, (firstn_length_le _ H);
+ reflexivity).
+- abstract
+(unfold fillReadFrame; cbn;
+ inversion_clear Hrp as [H|];
+ rewrite rev_involutive, firstn_skipn;
+ reflexivity).
+Defined.
+
+Lemma Bwd_ctx_correct l ctx : Bwd_ctx (length l)
+  (fillReadFrame ctx {| prevData := rev l
+                      ; nextData := nil
+                      |})
+  = Some (exist _ (l, ctx) (conj (refl_equal _) (refl_equal _))).
+Proof.
+cbn.
+destruct (Nat.leb_spec (length l) (length (rev l ++ prevData (activeReadFrame ctx)))) as [H0|H0];
+ [|elim (Lt.lt_not_le _ _ H0); rewrite app_length, rev_length; auto with arith].
+set (H := (Bwd_ctx_subproof _ _ _)).
+generalize H; clear H.
+set (H := (Bwd_ctx_subproof0 _ _ _ _ _ _ _)).
+generalize H; clear H.
+rewrite firstn_app.
+replace (firstn (length l) (rev l)) with (rev l) by
+ (rewrite <- rev_length, firstn_all; reflexivity).
+replace (firstn (length l - length (rev l)) _) with (@nil Cell) by
+ (rewrite rev_length, Nat.sub_diag; reflexivity).
+replace (skipn (length l) _) with (prevData (activeReadFrame ctx)) by
+ (apply (app_inv_head (firstn (length l) (rev l ++ prevData (activeReadFrame ctx))));
+  rewrite <- rev_length, firstn_skipn, firstn_app, firstn_all, Nat.sub_diag; cbn;
+  rewrite app_nil_r; reflexivity).
+rewrite app_nil_r, (rev_involutive l).
+intros H; elim H using (K_dec_set State_dec); clear H.
+apply (K_dec_set Nat.eq_dec).
+destruct ctx as [irf [rp rn] [wd we] iwf].
+reflexivity.
+Qed.
+
+Local Open Scope thrist_scope.
+
+Notation "x ~~> y" := (MachineCode.T x y) (at level 70) : type_scope.
+Notation "x ->> y" := (Thrst MachineCode.T x y) (at level 70) : type_scope.
+
+Definition Program := forall x : State, option { y : State & x ->> y }.
+
+Definition crash : Program :=
+  fun x => None.
+
+Definition nop : Program :=
+  fun x => Some (existT _ x []).
+
+Definition newFrame (n : nat) : Program :=
+  fun x => Some (existT _ _ (MachineCode.NewFrame n x <| [])).
+
+Definition moveFrame : Program.
+intros s.
+destruct (MoveFrame_ctx s) as [P|];[left|right].
+destruct P as [[l ctx] Hs].
+exact (existT _ _ (eq_nil Hs |> MachineCode.MoveFrame l ctx)).
+Defined.
+
+Lemma moveFrame_correct : forall l ctx, moveFrame
+  {| inactiveReadFrames := inactiveReadFrames ctx
+   ; activeReadFrame := activeReadFrame ctx
+   ; activeWriteFrame := fullWriteFrame l
+   ; inactiveWriteFrames := activeWriteFrame ctx :: inactiveWriteFrames ctx
+   |} = Some (existT _ _ (MachineCode.MoveFrame l ctx <| [])).
+Proof.
+intros l ctx.
+unfold moveFrame.
+rewrite MoveFrame_ctx_correct.
+reflexivity.
+Qed.
+
+Definition dropFrame : Program.
+intros s.
+destruct (DropFrame_ctx s) as [P|];[left|right].
+destruct P as [[rf ctx] Hs].
+exact (existT _ _ (eq_nil Hs |> MachineCode.DropFrame rf ctx)).
+Defined.
+
+Lemma dropFrame_correct : forall rf ctx, dropFrame
+  {| inactiveReadFrames := activeReadFrame ctx :: inactiveReadFrames ctx
+   ; activeReadFrame := rf
+   ; activeWriteFrame := activeWriteFrame ctx
+   ; inactiveWriteFrames := inactiveWriteFrames ctx
+   |} = Some (existT _ _ (MachineCode.DropFrame rf ctx <| [])).
+Proof.
+intros l ctx.
+unfold dropFrame.
+rewrite DropFrame_ctx_correct.
+reflexivity.
+Qed.
+
+Definition write (b : bool) : Program.
+intros s.
+destruct (Write_ctx s) as [P|];[left|right].
+destruct P as [ctx Hs].
+exact (existT _ _ (eq_nil Hs |> MachineCode.Write b ctx)).
+Defined.
+
+Lemma write_correct : forall b ctx, write b
+  (fillContext ctx {| readLocalState := nil
+                    ; writeLocalState := newWriteFrame 1
+                    |}) = Some (existT _ _ (MachineCode.Write b ctx <| [])).
+Proof.
+intros l ctx.
+unfold write.
+rewrite Write_ctx_correct.
+reflexivity.
+Qed.
+
+Definition skip (n : nat) : Program.
+intros s.
+destruct (Skip_ctx n s) as [P|];[left|right].
+destruct P as [ctx Hs].
+exact (existT _ _ (eq_nil Hs |> MachineCode.Skip n ctx)).
+Defined.
+
+Lemma skip_correct : forall n ctx, skip n
+  (fillContext ctx {| readLocalState := nil
+                    ; writeLocalState := newWriteFrame n
+                    |}) = Some (existT _ _ (MachineCode.Skip n ctx <| [])).
+Proof.
+intros l ctx.
+unfold skip.
+rewrite Skip_ctx_correct.
+reflexivity.
+Qed.
+
+Definition copy (n : nat) : Program.
+intros s.
+destruct (Copy_ctx n s) as [P|];[left|right].
+destruct P as [[l ctx] [_ Hs]].
+exact (existT _ _ (eq_nil Hs |> MachineCode.Copy l ctx)).
+Defined.
+
+Lemma copy_correct : forall l ctx, copy (length l)
+  (fillContext ctx {| readLocalState := l
+                    ; writeLocalState := newWriteFrame (length l)
+                    |}) = Some (existT _ _ (MachineCode.Copy l ctx <| [])).
+Proof.
+intros l ctx.
+unfold copy.
+rewrite Copy_ctx_correct.
+reflexivity.
+Qed.
+
+Definition fwd (n : nat) : Program.
+intros s.
+destruct (Fwd_ctx n s) as [P|];[left|right].
+destruct P as [[l ctx] [_ Hs]].
+exact (existT _ _ (eq_nil Hs |> MachineCode.Fwd l ctx)).
+Defined.
+
+Lemma fwd_correct : forall l ctx, fwd (length l)
+  (fillReadFrame ctx {| prevData := nil
+                      ; nextData := l
+                      |}) = Some (existT _ _ (MachineCode.Fwd l ctx <| [])).
+Proof.
+intros l ctx.
+unfold fwd.
+rewrite Fwd_ctx_correct.
+reflexivity.
+Qed.
+
+Definition bwd (n : nat) : Program.
+intros s.
+destruct (Bwd_ctx n s) as [P|];[left|right].
+destruct P as [[l ctx] [_ Hs]].
+exact (existT _ _ (eq_nil Hs |> MachineCode.Bwd l ctx)).
+Defined.
+
+Lemma bwd_correct : forall l ctx, bwd (length l)
+  (fillReadFrame ctx {| prevData := rev l
+                      ; nextData := nil
+                      |}) = Some (existT _ _ (MachineCode.Bwd l ctx <| [])).
+Proof.
+intros l ctx.
+unfold bwd.
+rewrite Bwd_ctx_correct.
+reflexivity.
+Qed.
+
+Definition seq (p1 p2 : Program) : Program.
+intros x.
+destruct (p1 x) as [[y thr1]|];[|exact None].
+destruct (p2 y) as [[z thr2]|];[|exact None].
+exact (Some (existT _ _ (thr1 |><| thr2))).
+Defined.
+Notation "p1 ;;; p2" := (seq p1 p2) (at level 40, left associativity) : mc_scope.
+
+Definition choice (p1 p2 : Program) : Program.
+intros x.
+destruct (nextData (activeReadFrame x)) as [|[b|] tl];[exact None| |exact None].
+exact ((if b then p2 else p1) x).
+Defined.
+Notation "p1 ||| p2" := (choice p1 p2) (at level 50, left associativity) : mc_scope.
+
+Local Open Scope mc_scope.
+
+Definition bump n p : Program := fwd n ;;; p ;;; bwd n.
+
+Definition runMachine (p : Program) (s : State) : option State :=
+option_map (@projT1 _ _) (p s).
+
+Lemma runMachine_seq (p1 p2 : Program) (s : State) :
+ runMachine (p1 ;;; p2) s = option_bind (runMachine p2) (runMachine p1 s).
+Proof.
+unfold runMachine, seq.
+destruct (p1 s) as [[s0 thr0]|];[|reflexivity].
+cbn.
+destruct (p2 s0) as [[s1 thr1]|];reflexivity.
+Qed.
+
+Lemma runMachine_choice (p1 p2 : Program) (s : State) :
+ runMachine (p1 ||| p2) s = match nextData (activeReadFrame s) with
+ | Some b :: _ => runMachine (if b then p2 else p1) s
+ | _ => None
+ end.
+Proof.
+destruct s as [irf [rp [|[|] tl]] awf iwf]; reflexivity.
+Qed.
+
+Lemma runMachine_bump (p : Program) l ctx0 ctx1 :
+ runMachine p
+   (fillReadFrame ctx0 {| prevData := rev l; nextData := nil |}) =
+   Some (fillReadFrame ctx1 {| prevData := rev l; nextData := nil |}) ->
+ runMachine (bump (length l) p)
+   (fillReadFrame ctx0 {| prevData := nil; nextData := l |}) =
+   Some (fillReadFrame ctx1 {| prevData := nil; nextData := l |}).
 Proof.
 intros Hp.
 unfold bump.
-repeat rewrite runMachine_append.
-unfold fillContext.
-simpl (runMachine (fwd _) _).
-unfold State.fwd, oModActiveReadFrame.
-simpl (option_map _ _).
-rewrite <- app_assoc, fwdFrame_correct.
-unfold option_bind at 2; simpl (option_join _).
-change (runMachine p _) with (runMachine p (fillContext (bumpContext ctx l) ls1)).
-rewrite Hp.
-unfold option_bind; cbn.
-unfold State.bwd, oModActiveReadFrame; cbn.
-rewrite <- rev_length, bwdFrame_correct, rev_involutive, <- app_assoc.
+repeat rewrite runMachine_seq.
+unfold runMachine at 3.
+rewrite fwd_correct; cbn.
+rewrite Hp; cbn.
+unfold runMachine.
+rewrite bwd_correct.
 reflexivity.
 Qed.
